Split int, vldata into code and proof

examples/lowparse/LowParse.BigEndian.fst
@@ -4,6 +4,7 @@ open FStar.Mul
 
 module Seq = FStar.Seq
 module U8 = FStar.UInt8
+module U32 = FStar.UInt32
 
 let be_to_n_1_spec
   (s: Seq.seq U8.t { Seq.length s == 1 } )
@@ -63,3 +64,66 @@ let n_to_be'_spec
     Seq.index (n_to_be' len n) (len - 1) == n % 256
   ))
 = Seq.lemma_eq_intro (n_to_be' (len - 1) (n / 256)) (Seq.slice (n_to_be' len n) 0 (len - 1))
+
+let rec index_n_to_be
+  (len: U32.t)
+  (n: nat { n < pow2 (Prims.op_Multiply 8 (U32.v len)) } )
+  (i: nat {i < U32.v len})
+: Lemma
+  (requires True)
+  (ensures (U8.v (Seq.index (n_to_be len n) i) == Seq.index (n_to_be' (U32.v len) n) i))
+  (decreases (U32.v len))
+= n_to_be_spec len n;
+  n_to_be'_spec (U32.v len) n;
+  if i = U32.v len - 1
+  then ()
+  else begin
+    let len' = U32.sub len 1ul in
+    let n' = n / 256 in
+    Seq.lemma_index_slice (n_to_be len n) 0 (U32.v len - 1) i;
+    Seq.lemma_index_slice (n_to_be' (U32.v len) n) 0 (U32.v len - 1) i;
+    index_n_to_be len' n' i
+  end
+
+let rec div_256
+  (n: nat)
+  (times: nat)
+: GTot nat
+  (decreases times)
+= if times = 0
+  then n % 256
+  else div_256 (n / 256) (times - 1)
+
+let rec index_n_to_be'
+  (len: nat)
+  (n: nat)
+  (i: nat {i < len})
+: Lemma
+  (requires True)
+  (ensures (Seq.index (n_to_be' len n) i == div_256 n (len - 1 - i)))
+  (decreases len)
+= n_to_be'_spec len n;
+  if i = len - 1
+  then ()
+  else index_n_to_be' (len - 1) (n / 256) i
+
+let lemma_u8_eq_intro
+  (s1 s2: bytes)
+  (u: unit { Seq.length s1 == Seq.length s2 } )
+  (f: (
+    (i: nat) ->
+    Lemma
+    (requires (i < Seq.length s1))
+    (ensures (U8.v (Seq.index s1 i) == U8.v (Seq.index s2 i)))
+  ))
+: Lemma
+  (ensures (s1 == s2))
+= let g
+    (i: nat { i < Seq.length s1 } )
+  : Lemma
+    (Seq.index s1 i == Seq.index s2 i)
+  = f i;
+    U8.v_inj (Seq.index s1 i) (Seq.index s2 i)
+  in
+  Classical.forall_intro g;
+  Seq.lemma_eq_intro s1 s2
