examples/lowparse/LowParse.SLow.VLData.fst
@@ -1,7 +1,5 @@
 module LowParse.SLow.VLData
-include LowParse.Spec.VLData
-include LowParse.SLow.FLData
-include LowParse.SLow.Int
+include LowParse.SLow.VLData.Proof
 
 module Seq = FStar.Seq
 module U8 = FStar.UInt8
@@ -11,47 +9,6 @@ module E = LowParse.BigEndian
 module Cast = FStar.Int.Cast
 module B32 = FStar.Bytes
 
-#reset-options "--z3cliopt smt.arith.nl=false --z3rlimit 128 --max_ifuel 64 --max_fuel 64"
-
-let pow2_8 () : Lemma (pow2 8 == 256) [SMTPat (pow2 8)] = assert_norm (pow2 8 == 256)
-let pow2_16 () : Lemma (pow2 16 == 65536) [SMTPat (pow2 16)] = assert_norm (pow2 16 == 65536)
-let pow2_24 () : Lemma (pow2 24 == 16777216) [SMTPat (pow2 24)] = assert_norm (pow2 24 == 16777216)
-let pow2_32 () : Lemma (pow2 32 == 4294967296) [SMTPat (pow2 32)] = assert_norm (pow2 32 == 4294967296)
-
-let serialize_bounded_integer_1_spec
-  (input: bounded_integer 1)
-: Lemma
-  (let ser = serialize (serialize_bounded_integer 1) input in
-   Seq.length ser == 1 /\
-   U8.v (Seq.index ser 0) == U32.v input % 256
-  )
-= index_n_to_be 1ul (U32.v input) 0
-
-let serialize32_bounded_integer_1'
-  (buf: B32.lbytes 1)
-  (input: bounded_integer 1)
-: Tot (B32.lbytes 1)
-= let byte0 = Cast.uint32_to_uint8 input in
-  let buf0 = B32.set_byte buf 0ul byte0 in
-  buf0
-
-let serialize32_bounded_integer_1_correct
-  (buf: B32.lbytes 1)
-  (input: bounded_integer 1)
-: Lemma
-  (serializer32_correct (serialize_bounded_integer 1) input (serialize32_bounded_integer_1' buf input))
-= let ser32 = serialize32_bounded_integer_1' buf input in
-  let rser32 = B32.reveal ser32 in
-  let byte0 = Cast.uint32_to_uint8 input in
-  assert (U8.v byte0 == U32.v input % 256);
-  assert (Seq.index rser32 0 == byte0);
-  serialize_bounded_integer_1_spec input;
-  let ser = serialize (serialize_bounded_integer 1) input in
-  assert (Seq.length ser == 1);
-  lemma_u8_eq_intro rser32 ser ()
-    (fun (i: nat) -> if i = 0 then () else ());
-  assert (serializer32_correct (serialize_bounded_integer 1) input ser32)
-
 inline_for_extraction
 let serialize32_bounded_integer_1 : serializer32 (serialize_bounded_integer 1) =
   (fun (input: bounded_integer 1) -> ((
@@ -60,51 +17,6 @@ let serialize32_bounded_integer_1 : serializer32 (serialize_bounded_integer 1) =
     serialize32_bounded_integer_1' b input
   ) <: (res: B32.bytes { serializer32_correct (serialize_bounded_integer 1) input res } )))
 
-let serialize_bounded_integer_2_spec
-  (input: bounded_integer 2)
-: Lemma
-  (let ser = serialize (serialize_bounded_integer 2) input in
-   Seq.length ser == 2 /\
-   U8.v (Seq.index ser 1) == U32.v input % 256 /\
-   U8.v (Seq.index ser 0) == (U32.v input / 256) % 256
-  )
-= index_n_to_be 2ul (U32.v input) 1;
-  index_n_to_be 2ul (U32.v input) 0
-
-let serialize32_bounded_integer_2'
-  (buf: B32.lbytes 2)
-  (input: bounded_integer 2)
-: Tot (B32.lbytes 2)
-= let byte1 = Cast.uint32_to_uint8 input in
-  let byte0v = U32.div input 256ul in
-  let byte0 = Cast.uint32_to_uint8 byte0v in
-  let buf0 = B32.set_byte buf 0ul byte0 in
-  let buf1 = B32.set_byte buf0 1ul byte1 in
-  buf1
-
-#reset-options "--z3cliopt smt.arith.nl=false --z3rlimit 128 --max_ifuel 64 --max_fuel 64"
-
-let serialize32_bounded_integer_2_correct
-  (buf: B32.lbytes 2)
-  (input: bounded_integer 2)
-: Lemma
-  (serializer32_correct (serialize_bounded_integer 2) input (serialize32_bounded_integer_2' buf input))
-= let ser32 = serialize32_bounded_integer_2' buf input in
-  let rser32 = B32.reveal ser32 in
-  let byte1 = Cast.uint32_to_uint8 input in
-  assert (U8.v byte1 == U32.v input % 256);
-  assert (Seq.index rser32 1 == byte1);
-  let byte0v = U32.div input 256ul in
-  let byte0 = Cast.uint32_to_uint8 byte0v in
-  assert (U8.v byte0 == (U32.v input / 256) % 256);
-  assert (Seq.index rser32 0 == byte0);
-  serialize_bounded_integer_2_spec input;
-  let ser = serialize (serialize_bounded_integer 2) input in
-  assert (Seq.length ser == 2);
-  lemma_u8_eq_intro rser32 ser ()
-    (fun (i: nat) -> if i = 0 then () else if i = 1 then () else ());
-  assert (serializer32_correct (serialize_bounded_integer 2) input ser32)
-
 inline_for_extraction
 let serialize32_bounded_integer_2 : serializer32 (serialize_bounded_integer 2) =
   (fun (input: bounded_integer 2) -> ((
@@ -112,77 +24,6 @@ let serialize32_bounded_integer_2 : serializer32 (serialize_bounded_integer 2) =
     serialize32_bounded_integer_2_correct b input;
     serialize32_bounded_integer_2' b input
   ) <: (res: B32.bytes { serializer32_correct (serialize_bounded_integer 2) input res } )))
-
-let serialize_bounded_integer_3_spec
-  (input: bounded_integer 3)
-: Lemma
-  (let ser = serialize (serialize_bounded_integer 3) input in
-   Seq.length ser == 3 /\
-   U8.v (Seq.index ser 2) == U32.v input % 256 /\
-   U8.v (Seq.index ser 1) == (U32.v input / 256) % 256 /\
-   U8.v (Seq.index ser 0) == ((U32.v input / 256) / 256) % 256
-  )
-= let ser = serialize (serialize_bounded_integer 3) input in
-  assert (Seq.length ser == 3);
-  let f2 () : Lemma (U8.v (Seq.index ser 2) == U32.v input % 256) =
-    index_n_to_be 3ul (U32.v input) 2;
-    index_n_to_be' 3 (U32.v input) 2 
-  in
-  f2 ();
-  let f1 () : Lemma (U8.v (Seq.index ser 1) == (U32.v input / 256) % 256) =
-    index_n_to_be 3ul (U32.v input) 1;
-    index_n_to_be' 3 (U32.v input) 1
-  in
-  f1 ();
-  let f0 () : Lemma (U8.v (Seq.index ser 0) == ((U32.v input / 256) / 256) % 256) =
-    index_n_to_be 3ul (U32.v input) 0;
-    index_n_to_be' 3 (U32.v input) 0;
-    assert (U8.v (Seq.index ser 0) == div_256 (U32.v input) 2);
-    assert_norm (div_256 (U32.v input) 2 == ((U32.v input / 256) / 256) % 256);
-    assert (U8.v (Seq.index ser 0) == ((U32.v input / 256) / 256) % 256)
-  in
-  f0 ()
-
-let serialize32_bounded_integer_3'
-  (buf: B32.lbytes 3)
-  (input: bounded_integer 3)
-: Tot (B32.lbytes 3)
-= let byte2 = Cast.uint32_to_uint8 input in
-  let byte1v = U32.div input 256ul in
-  let byte1 = Cast.uint32_to_uint8 byte1v in
-  let byte0v = U32.div byte1v 256ul in
-  let byte0 = Cast.uint32_to_uint8 byte0v in
-  let buf0 = B32.set_byte buf 0ul byte0 in
-  let buf1 = B32.set_byte buf0 1ul byte1 in
-  let buf2 = B32.set_byte buf1 2ul byte2 in
-  buf2
-
-#reset-options "--z3cliopt smt.arith.nl=false --z3rlimit 256 --max_ifuel 64 --max_fuel 64"
-
-let serialize32_bounded_integer_3_correct
-  (buf: B32.lbytes 3)
-  (input: bounded_integer 3)
-: Lemma
-  (serializer32_correct (serialize_bounded_integer 3) input (serialize32_bounded_integer_3' buf input))
-= let ser32 = serialize32_bounded_integer_3' buf input in
-  let rser32 = B32.reveal ser32 in
-  let byte2 = Cast.uint32_to_uint8 input in
-  assert (U8.v byte2 == U32.v input % 256);
-  assert (Seq.index rser32 2 == byte2);
-  let byte1v = U32.div input 256ul in
-  let byte1 = Cast.uint32_to_uint8 byte1v in
-  assert (U8.v byte1 == (U32.v input / 256) % 256);
-  assert (Seq.index rser32 1 == byte1);
-  let byte0v = U32.div byte1v 256ul in
-  let byte0 = Cast.uint32_to_uint8 byte0v in
-  assert (U8.v byte0 == ((U32.v input / 256) / 256) % 256);
-  assert (Seq.index rser32 0 == byte0);
-  serialize_bounded_integer_3_spec input;
-  let ser = serialize (serialize_bounded_integer 3) input in
-  assert (Seq.length ser == 3);
-  lemma_u8_eq_intro rser32 ser ()
-    (fun (i: nat) -> if i = 0 then () else if i = 1 then () else if i = 2 then () else ());
-  assert (serializer32_correct (serialize_bounded_integer 3) input ser32)
 
 inline_for_extraction
 let serialize32_bounded_integer_3 : serializer32 (serialize_bounded_integer 3) =
@@ -209,28 +50,19 @@ inline_for_extraction
 let serialize32_bounded_integer
   (sz: integer_size)
 : Tot (serializer32 (serialize_bounded_integer sz))
-= assert (sz == 1 \/ sz == 2 \/ sz == 3 \/ sz == 4);
-  match sz with
+= match sz with
   | 1 -> serialize_bounded_integer_conv 1 sz serialize32_bounded_integer_1
   | 2 -> serialize_bounded_integer_conv 2 sz serialize32_bounded_integer_2
   | 3 -> serialize_bounded_integer_conv 3 sz serialize32_bounded_integer_3
   | 4 -> serialize_bounded_integer_conv 4 sz serialize32_bounded_integer_4
 
-#reset-options "--z3rlimit 32"
-
 inline_for_extraction
 let decode32_bounded_integer_1
  (b: B32.lbytes 1)
 : Tot (y: bounded_integer 1 { y == decode_bounded_integer 1 (B32.reveal b) } )
-= let r = B32.get b 0ul in
-  assert (r == B32.index b 0);
-  B32.index_reveal b 0;
-  E.be_to_n_1_spec (B32.reveal b);
-  let res : U32.t = Cast.uint8_to_uint32 r in
-  assert (res == (decode_bounded_integer 1 (B32.reveal b) <: U32.t));
-  assert (U32.v res < pow2 (FStar.Mul.op_Star 8 1));
-  let (res: bounded_integer 1) = res in
-  (res <: (y: bounded_integer 1 { y == decode_bounded_integer 1 (B32.reveal b) }))
+= let r = decode32_bounded_integer_1' b in
+  decode32_bounded_integer_1_correct b;
+  (r <: (r: bounded_integer 1 { r == decode_bounded_integer 1 (B32.reveal b) } ))
 
 inline_for_extraction
 let parse32_bounded_integer_1 : parser32 (parse_bounded_integer 1) =
@@ -240,39 +72,6 @@ let parse32_bounded_integer_1 : parser32 (parse_bounded_integer 1) =
     ()
     (decode32_bounded_integer_1)
 
-let synth_bounded_integer_2
-  (x: U16.t)
-: GTot (bounded_integer 2)
-= Cast.uint16_to_uint32 x
-
-let synth_bounded_integer_2_inj
-  ()
-: Lemma
-  (forall (x x' : U16.t) . synth_bounded_integer_2 x == synth_bounded_integer_2 x' ==> x == x')
-= ()
-
-#reset-options "--z3rlimit 256 --max_fuel 64 --max_ifuel 64"
-
-let parse_bounded_integer_2_spec
-  ()
-: Lemma
-  (forall (input: bytes) . parse (parse_bounded_integer 2) input == parse (parse_u16 `parse_synth` synth_bounded_integer_2) input)
-= let f
-    (input: bytes { Seq.length input == 2 })
-  : Lemma
-    ((decode_u16 `compose` synth_bounded_integer_2) input == decode_bounded_integer 2 input)
-  = E.be_to_n_2_spec input;
-    E.lemma_be_to_n_is_bounded input;
-    assert (U16.v (decode_u16 input) == U32.v (decode_bounded_integer 2 input));
-    assert (U32.v ((decode_u16 `compose` synth_bounded_integer_2) input) == U32.v (decode_bounded_integer 2 input));
-    U32.v_inj ((decode_u16 `compose` synth_bounded_integer_2) input) (decode_bounded_integer 2 input)
-  in
-  Classical.forall_intro f;
-  decode_u16_injective ();
-  synth_bounded_integer_2_inj ();
-  make_total_constant_size_parser_compose 2 U16.t (bounded_integer 2) (decode_u16) (synth_bounded_integer_2);
-  assert_norm (forall (input: bytes) . parse (parse_bounded_integer 2) input == parse (make_total_constant_size_parser 2 (bounded_integer 2) (decode_u16 `compose` synth_bounded_integer_2)) input)
-
 inline_for_extraction
 let parse32_bounded_integer_2 : parser32 (parse_bounded_integer 2) =
   fun (input: bytes32) -> (
@@ -281,64 +80,13 @@ let parse32_bounded_integer_2 : parser32 (parse_bounded_integer 2) =
     (res <: (res: option (bounded_integer 2 * U32.t) { parser32_correct (parse_bounded_integer 2) input res} ))
   )
 
-(*
-inline_for_extraction
-let decode32_bounded_integer_2
- (b: B32.lbytes 2)
-: Tot (y: bounded_integer 2 { y == decode_bounded_integer 2 (B32.reveal b) } )
-= let b0r = B32.get b 0ul in
-  assert (b0r == B32.index b 0);
-  B32.index_reveal b 0;
-  let b0 = Cast.uint8_to_uint32 b0r in
-  let b1r = B32.get b 1ul in
-  assert (b1r == B32.index b 1);
-  B32.index_reveal b 1;
-  let b1 = Cast.uint8_to_uint32 b1r in
-  let res = U32.add b1 (U32.mul 256ul b0) in
-  E.be_to_n_2_spec (B32.reveal b);
-  E.lemma_be_to_n_is_bounded (B32.reveal b);
-  assert (res == (decode_bounded_integer 2 (B32.reveal b) <: U32.t));
-  assert (U32.v res < pow2 (FStar.Mul.op_Star 8 2));
-  let (res: bounded_integer 2) = res in
-  (res <: (y: bounded_integer 2 { y == decode_bounded_integer 2 (B32.reveal b) }))
-
-inline_for_extraction
-let parse32_bounded_integer_2 : parser32 (parse_bounded_integer 2) =
-  decode_bounded_integer_injective 2;
-  make_total_constant_size_parser32 2 2ul
-    (decode_bounded_integer 2)
-    ()
-    (decode32_bounded_integer_2)
-*)
-
-#reset-options "--z3rlimit 1024 --z3refresh  --smtencoding.elim_box true --smtencoding.l_arith_repr native --smtencoding.nl_arith_repr wrapped --max_fuel 64 --max_ifuel 64"
-
 inline_for_extraction
 let decode32_bounded_integer_3
  (b: B32.lbytes 3)
 : Tot (y: bounded_integer 3 { y == decode_bounded_integer 3 (B32.reveal b) } )
-= let b0r = B32.get b 0ul in
-  assert (b0r == B32.index b 0);
-  B32.index_reveal b 0;
-  let b0 = Cast.uint8_to_uint32 b0r in
-  let b1r = B32.get b 1ul in
-  assert (b1r == B32.index b 1);
-  B32.index_reveal b 1;
-  let b1 = Cast.uint8_to_uint32 b1r in
-  let b2r = B32.get b 2ul in
-  assert (b2r == B32.index b 2);
-  B32.index_reveal b 2;
-  let b2 = Cast.uint8_to_uint32 b2r in
-  let res = U32.add b2 (U32.mul 256ul (U32.add b1 (U32.mul 256ul b0))) in
-  E.be_to_n_3_spec (B32.reveal b);
-  E.lemma_be_to_n_is_bounded (B32.reveal b);
-  assert (U32.v res == U32.v (decode_bounded_integer 3 (B32.reveal b) <: U32.t));
-  U32.v_inj res (decode_bounded_integer 3 (B32.reveal b) <: U32.t);
-  assert (U32.v res < pow2 (FStar.Mul.op_Star 8 3));
-  let (res: bounded_integer 3) = res in
-  (res <: (y: bounded_integer 3 { y == decode_bounded_integer 3 (B32.reveal b) }))
-
-#reset-options "--z3rlimit 256 --max_fuel 64 --max_ifuel 64"
+= let r = decode32_bounded_integer_3' b in
+  decode32_bounded_integer_3_correct b;
+  (r <: (r: bounded_integer 3 { r == decode_bounded_integer 3 (B32.reveal b) } ))
 
 inline_for_extraction
 let parse32_bounded_integer_3 : parser32 (parse_bounded_integer 3) =
@@ -348,20 +96,6 @@ let parse32_bounded_integer_3 : parser32 (parse_bounded_integer 3) =
     ()
     (decode32_bounded_integer_3)
 
-let synth_bounded_integer_4
-  (x: U32.t)
-: GTot (bounded_integer 4)
-= x
-
-let parse_bounded_integer_4_spec
-  ()
-: Lemma
-  (forall (input: bytes) . parse (parse_bounded_integer 4) input == parse (parse_u32 `parse_synth` synth_bounded_integer_4) input)
-= assert (forall (input: bytes { Seq.length input == 4 }) . (decode_u32 `compose` synth_bounded_integer_4) input == decode_bounded_integer 4 input);
-  decode_u32_injective ();
-  make_total_constant_size_parser_compose 4 U32.t (bounded_integer 4) (decode_u32) (synth_bounded_integer_4);
-  assert_norm (forall (input: bytes) . parse (parse_bounded_integer 4) input == parse (make_total_constant_size_parser 4 (bounded_integer 4) (decode_u32 `compose` synth_bounded_integer_4)) input)
-
 inline_for_extraction
 let parse32_bounded_integer_4 : parser32 (parse_bounded_integer 4) =
   fun (input: bytes32) -> (
@@ -369,6 +103,26 @@ let parse32_bounded_integer_4 : parser32 (parse_bounded_integer 4) =
     parse_bounded_integer_4_spec ();
     (res <: (res: option (bounded_integer 4 * U32.t) { parser32_correct (parse_bounded_integer 4) input res} ))
   )
+
+inline_for_extraction
+let parse_bounded_integer_conv
+  (sz sz' : integer_size)
+  (s32: parser32 (parse_bounded_integer sz))
+: Pure (parser32 (parse_bounded_integer sz'))
+  (requires (sz == sz'))
+  (ensures (fun _ -> True))
+= s32
+
+inline_for_extraction
+let parse32_bounded_integer
+  (i: integer_size)
+: Tot (parser32 (parse_bounded_integer i))
+= integer_size_values i;
+  match i with
+  | 1 -> parse_bounded_integer_conv 1 i parse32_bounded_integer_1
+  | 2 -> parse_bounded_integer_conv 2 i parse32_bounded_integer_2
+  | 3 -> parse_bounded_integer_conv 3 i parse32_bounded_integer_3
+  | 4 -> parse_bounded_integer_conv 4 i parse32_bounded_integer_4
 
 (* Parsers and serializers for the payload *)
 
